examples/Online_with_authn/DY.OnlineA.Properties.fst
@@ -9,6 +9,8 @@ open DY.Extend
 open DY.OnlineA.Data
 open DY.OnlineA.Invariants
 
+#set-options "--fuel 0 --ifuel 1 --z3rlimit 25  --z3cliopt 'smt.qi.eager_threshold=100'"
+
 /// This is the new property, we want to show:
 /// if Alice finishes a run identified by Bob and a nonce n_a,
 /// then this Bob was involved in the run,
@@ -17,19 +19,21 @@ open DY.OnlineA.Invariants
 
 val responder_authentication:
   tr:trace -> 
-  alice:principal -> bob:principal ->
+  ts:timestamp ->
+  alice:principal -> sid:state_id 
+  -> bob:principal ->
   n_a:bytes ->
   Lemma
   (requires
      trace_invariant tr /\
-     state_was_set_some_id tr alice (ReceivedAck {bob; n_a})
+     // state_was_set_some_id tr alice (ReceivedAck {bob; n_a})
+     state_was_set_at tr ts alice sid (ReceivedAck {bob; n_a})
   )
   (ensures
-     is_corrupt tr (principal_label alice) \/ is_corrupt tr (principal_label bob) \/
-     state_was_set_some_id tr bob (SendingAck {alice; n_a})
+     is_corrupt (prefix tr ts) (principal_label alice) \/ is_corrupt (prefix tr ts) (principal_label bob) \/
+     state_was_set_some_id (prefix tr ts) bob (SendingAck {alice; n_a})
   )
-let responder_authentication tr alice bob n_a = ()
-
+let responder_authentication tr ts alice sid bob n_a = ()
 
 /// We still have nonce secrecy:
 
